some fixes to the modelling, changing the way we use indices

examples/crypto/HyE.AE.fst
@@ -14,7 +14,6 @@ open CoreCrypto
 
 module B = Platform.Bytes
 
-// Import HyE.PlainAE later, so we have that Plain.t is actually of type bytes.
 open HyE.PlainAE
 
 let ivsize = aeadRealIVSize AES_128_GCM
@@ -24,44 +23,46 @@ type msg = protected_ae_plain
 type cipher = b:bytes{B.length b >= ivsize}
 (* MK: minimal cipher length twice blocksize? *)
 
-type log_t (r:rid) = m_rref r (seq (msg * cipher)) grows
+type log_t (i:id) (r:rid) = m_rref r (seq ((msg i) * cipher)) grows
 
-noeq abstract type key =
-  | Key: #i:id -> #region:rid -> raw:aes_key -> log:log_t region -> honest:bool-> key
+(**
+   The key type is abstract and can only be accessed via the leak and coerce_key functions.
+*)
+noeq abstract type key (i:id) =
+  | Key: #region:rid -> raw:aes_key -> log:log_t i region -> honest:bool-> (key i)
 
-val getIndex: k:key -> Tot id
-let getIndex k =
-  k.i
-
-let safe_key_gen parent m0 (k:key) m1 =
+(** 
+    safe_key_gen makes sure that memory safety is preserved while generating a key.
+    Also, it makes sure that the log created along with the key is empty.
+*)
+let safe_key_gen #i parent m0 (k:key i) m1 =
     modifies Set.empty m0 m1
   /\ extends k.region parent
   /\ fresh_region k.region m0.h m1.h
   /\ m_contains k.log m1
+  /\ m_sel m1 k.log == createEmpty
 
 (**
    This function generates a key in a fresh region of memory below the parent region.
    The postcondition ensures that the log is empty after creation.
 *)
-val keygen: i:id -> parent:rid -> ST key
+val keygen: #i:id -> parent:rid -> ST (key i)
   (requires (fun _ -> True))
   (ensures  (fun h0 k h1 -> 
     safe_key_gen parent h0 k h1
-    /\ m_sel h1 k.log == createEmpty
-    ))
-
-let keygen i parent =
+  ))
+let keygen #i parent =
   let raw = random keysize in
   let region = new_region parent in
   let log = alloc_mref_seq region createEmpty in
   Key #i #region raw log true
 
 (**
-   The leak function transforms an abstract key into a raw aes_key.
+   The leak_key function transforms an abstract key into a raw aes_key.
    The refinement type on the key makes sure that no honest keys can be leaked.
 *)
-val leak: k:key{not (honest k.i)} -> Tot aes_key 
-let leak k =
+val leak_key: #i:id -> k:key i{not (honest i)} -> Tot aes_key 
+let leak_key #i k =
   k.raw
 
 (**
@@ -69,7 +70,7 @@ let leak k =
    as we need to allocate space in memory for the key. The refinement type on the key makes sure that
    abstract keys created this way can not be honest.
 *)
-val coerce_key: i:id{not (honest i) } -> parent:rid -> aes_key -> ST key
+val coerce_key: i:id{not (honest i) } -> parent:rid -> aes_key -> ST (key i)
   (requires (fun _ -> True))
   (ensures  (safe_key_gen parent))
 let coerce_key i parent raw = 
@@ -77,37 +78,44 @@ let coerce_key i parent raw =
   let log = alloc_mref_seq region createEmpty in
   Key #i #region raw log false
 
-type safe_log_append k fst h0 snd h1 =
+(**
+   safe_log_append makes sure that new entries added to the log are appended in a memory-safe way.
+*)
+type safe_log_append k entry h0 h1 =
     modifies_one k.region h0 h1 
     /\ m_contains k.log h1
-    /\ m_sel h1 k.log == snoc (m_sel h0 k.log) (fst, snd)
-    /\ witnessed (at_least (Seq.length (m_sel h0 k.log)) (fst, snd) k.log)
-
-// Should the precondition not be guaranteed by the key type? Same thing in decrypt.
-val encrypt: k:key -> m:msg -> ST cipher
-  (requires (fun h0 -> 
-    getIndex k = PlainAE.getIndex m(*m_contains k.log h0*)))
-  (ensures  (safe_log_append k m))
-
-(* There is currently no check for int-ctxt*)
-let encrypt k m : cipher =
+    /\ m_sel h1 k.log == snoc (m_sel h0 k.log) entry
+    /\ witnessed (at_least (Seq.length (m_sel h0 k.log)) entry k.log)
+(**
+   Encrypt a a message under a key. Idealize if the key is honest and ae_ind_cca true.
+*)
+val encrypt: #(i:id) -> (k:key i) -> (m:msg i) -> ST cipher
+  (requires (fun h0 -> True
+    (*m_contains k.log h0*)))
+  (ensures  (fun h0 c h1 -> 
+    safe_log_append k (m,c) h0 h1 ))
+let encrypt #i k m : cipher =
   m_recall k.log;
   let iv = random ivsize in
-  let text = if (ae_ind_cca && honest k.i) then createBytes (length m) 0z else (repr m) in
-  let c = CoreCrypto.aead_encrypt AES_128_GCM k.raw iv empty_bytes text in
+  let p = if (ae_ind_cca && honest i) then createBytes (length m) 0z else (repr m) in
+  let c = CoreCrypto.aead_encrypt AES_128_GCM k.raw iv empty_bytes p in
   let c = iv@|c in
   write_at_end k.log (m,c);
   c
 
-
-val decrypt: k:key -> c:cipher -> ST (option msg)
+(**
+   Decrypt a ciphertext c using a key k. If the key is honest and ae_int_ctxt is idealized,
+   try to obtain the ciphertext from the log. Else decrypt via concrete implementation.
+   TODO: Make this a total function.
+*)
+val decrypt: #(i:id) -> (k:key i) -> c:cipher -> ST (option (msg i))
   (requires (fun h -> True (* Could require Map.contains h0 k.region *)))
   (ensures  (fun h0 res h1 -> //True))
     modifies_none h0 h1
-    /\ ( (b2t ae_int_ctxt /\ honest k.i /\ Some? res) ==> SeqProperties.mem (Some?.v res,c) (m_sel h0 k.log) )
+    /\ ( (b2t ae_int_ctxt /\ honest i /\ Some? res) ==> SeqProperties.mem (Some?.v res,c) (m_sel h0 k.log) )
     ))
-let decrypt k c =
-  if ae_int_ctxt && honest k.i then
+let decrypt #i k c =
+  if ae_int_ctxt && honest i then
     let log = m_read k.log in
     match seq_find (fun mc -> snd mc = c) log with
     | Some mc -> Some (fst mc)
@@ -117,6 +125,6 @@ let decrypt k c =
     assume( B.length c' >= aeadTagSize AES_128_GCM);
     let poption = (CoreCrypto.aead_decrypt AES_128_GCM k.raw iv empty_bytes c') in
     if Some? poption then
-      Some (PlainAE.coerce #k.i (Some?.v poption))
+      Some (PlainAE.coerce (Some?.v poption))
     else
       None
