examples/crypto/HyE.Flags.fsti
@@ -3,27 +3,24 @@
    both of AE and of PKE. The flags indicate whether certain assumption are assumed to be
    true or not. Also, the refinements on the flag type indicate implications between the
    assumptions such as ae_ind_cpa /\ ae_int_ctxt ==> ae_ind_cca.
-   Not that for purposes of type-checking, the flags are not set. This
+   Note, that for purposes of type-checking, the flags are not set. This
    ensures that the program is well typed for any permutation of set flags (that is permissible
    by the refinements).
+   TODO: Restrict access to functions for creation of ids?
 *)
 module HyE.Flags
 
 open HyE.Indexing
 
-//val pke_ind_cca : bool
-let pke_ind_cca = false
+val pke_ind_cca : bool
 
 val ae_int_ctxt : bool
-//let ae_int_ctxt = false
 
 val ae_ind_cpa : bool
 
 val ae_ind_cca : b:bool{ae_ind_cpa /\ ae_int_ctxt ==> b}
-//let ae_ind_cca = true
 
 val hpke_ind_cca : b:bool{b ==> b2t ae_ind_cca /\ pke_ind_cca}
-//let hpke_ind_cca = true
 
 val honest: i:id -> Tot bool
 
@@ -37,21 +34,6 @@ type dependentId =
     i:id{not (honest i)})
 
 val createId: unit -> Tot dependentId
-//val createId: unit -> Tot (i:id{pke_ind_cca ==> honest i})
-//val createId: unit -> Tot (i:id{honest i})
-
-(* Do we really need these? Better encode them in the types.*)
-//val ae_ind_cca_composition_lemma: unit -> Lemma
-//  (requires ae_ind_cpa /\ ae_int_ctxt)
-//  (ensures b2t ae_ind_cca)
-//
-//val ind_cca_composition_lemma: unit -> Lemma
-//  (requires b2t ae_ind_cca /\ pke_ind_cca)
-//  (ensures b2t hpke_ind_cca)
-//
-//val hpke_cca_implications_lemma: unit -> Lemma
-//  (requires b2t hpke_ind_cca)
-//  (ensures b2t ae_ind_cca /\ pke_ind_cca)
 
 val honest_implies_pke_inc_cca: i:id -> Lemma
   (requires honest i)
