examples/crypto/HyE.PKE.fst
@@ -1,3 +1,7 @@
+(**
+   TODO: - Documentation, some cleanup.
+	 - make decrypt a total function.
+*)
 module HyE.PKE  (* intuitively, parameterized by both PlainPKE and RSA *)
 
 open FStar.HyperHeap
@@ -8,53 +12,83 @@ open FStar.SeqProperties
 open FStar.Monotonic.Seq
 open FStar.List.Tot
 
+open CoreCrypto
+open Platform.Bytes
+
 open HyE.PlainPKE
 open HyE.Flags
 open HyE.RSA
 
-type cipher = RSA.cipher
-noeq type entry =
-  | Entry : c:RSA.cipher
-         -> p:protected_pke_plain
-         -> entry
 
+type cipher = RSA.cipher
+
+type msg = protected_pke_plain
 assume val ciphersize : nat
 
-type log_t (r:rid) = m_rref r (seq entry) grows
+type log_t (r:rid) = m_rref r (seq (msg*cipher)) grows
 
 noeq abstract type pkey = 
   | PKey: #region:rid -> rawpk:RSA.pkey -> log: log_t region -> pkey
 
-let access_pk_raw (pk:pkey) =
-  PKey?.rawpk pk
-
+val access_pk_raw: pkey -> Tot RSA.pkey
+let access_pk_raw pk =
+  pk.rawpk
 
 noeq abstract type skey =
-  | SKey: raw:RSA.skey -> pk:pkey -> skey
+  | SKey: rawsk:RSA.skey -> (pk:pkey)-> skey
 
-val keygen: parent:rid -> (pkey * skey)
+let safe_key_gen parent (pk:pkey) m0 m1 =
+    modifies Set.empty m0 m1
+    /\ m_contains pk.log m1
+    /\ extends pk.region parent
+    /\ fresh_region pk.region m0.h m1.h
+    /\ m_sel m1 pk.log == createEmpty
+
+val keygen: (parent:rid) -> ST (pkey * skey)
+  (requires (fun h -> True))
+  (ensures (fun h0 k h1 -> 
+  let (pk,sk) = k in
+  safe_key_gen parent pk h0 h1
+  ))
 let keygen parent  =
-  let pkey_raw, skey_raw = RSA.gen () in
+  let (pkey_raw, skey_raw) = (random RSA.pk_size),(random RSA.sk_size) in
   let region = new_region parent in
   let log = alloc_mref_seq region createEmpty in
   let pkey = PKey #region pkey_raw log in
-  pkey, SKey skey_raw pkey
+  let skey = SKey skey_raw pkey in
+  pkey, skey
+  
 
+type safe_log_append pk entry h0 h1 =
+    modifies_one pk.region h0 h1 
+    /\ m_contains pk.log h1
+    /\ m_sel h1 pk.log == snoc (m_sel h0 pk.log) entry
+    /\ witnessed (at_least (Seq.length (m_sel h0 pk.log)) entry pk.log)
 
-let encrypt pk (p:protected_pke_plain) : RSA.cipher =
-  let p' = if Flags.pke_ind_cca then RSA.dummy else PlainPKE.repr p in
+val encrypt: (pk:pkey) -> (p:protected_pke_plain) -> ST RSA.cipher
+  (requires (fun h0 -> True
+    (*m_contains k.log h0*)))
+  (ensures  (fun h0 c h1 ->
+    safe_log_append pk (p,c) h0 h1))
+let encrypt pk p =
+  m_recall pk.log;
+  let p' = if pke_ind_cca then createBytes (AE.keysize) 0z else PlainPKE.repr p in
   let c = RSA.enc pk.rawpk p' in
-  write_at_end pk.log (Entry c p);
+  write_at_end pk.log (p,c);
   c
 
-
-let decrypt sk (c:RSA.cipher) : option (protected_pke_plain) =
-  let log = m_read (PKey?.log sk.pk) in
-  match Flags.pke_ind_cca, seq_find (function Entry c' _ -> c=c') log with
-  | true,  Some t  -> Some(Entry?.p t)
-  | _,  _       ->
-    (match RSA.dec sk.raw c with
-     | Some t' -> 
-       let id = Flags.dishonestId() in
-       PlainPKE.coerce id sk.pk.region t'
-     | None     -> None)
+  
+val decrypt: (sk:skey) -> (c:RSA.cipher) -> ST (option (protected_pke_plain))
+  (requires (fun h -> True (* Could require Map.contains h0 k.region *)))
+  (ensures  (fun h0 p h1 -> True))
+    //modifies_none h0 h1))
+let decrypt sk c =
+  let log = m_read (sk.pk.log) in
+  let pke_p = seq_find (fun (_,c') -> c=c') log in
+    match pke_ind_cca,pke_p with
+    | true,Some (m,c)  -> Some(m)
+    | _,_ -> 
+      (match RSA.dec sk.rawsk c with
+	| Some p' ->
+	  Some (PlainPKE.coerce sk.pk.region p')
+	| None -> None)
