examples/crypto/HyE.PlainAE.fst
@@ -11,47 +11,47 @@ open Platform.Bytes
    If it is an honest message, it encapsulates a (protected) hpke payload.
    If it is not an hones message, it is plain bytes.
 *)
-type plain_content (i:id) = (
+type ae_plain_content (i:id) = (
   if honest i then
     protected_hpke_plain
   else 
     bytes
   )
 
-abstract type protected_ae_plain =
-  | Protected_ae_plain: #i:id -> p:plain_content i -> protected_ae_plain
-
-assume Plain_hasEq: hasEq protected_ae_plain
+abstract type protected_ae_plain (i:id)=
+  | Protected_ae_plain: (p:ae_plain_content i) -> protected_ae_plain i
 
 type ae_plain = bytes
 
-val ae_message_wrap: #i:id -> (p:plain_content i) -> protected_ae_plain
+(**
+   TODO: Review these functions and add pre-conditions?
+*)
+val ae_message_wrap: #i:id -> (p:ae_plain_content i) -> Tot (protected_ae_plain i)
 let ae_message_wrap #i p =
-  Protected_ae_plain #i p
+  Protected_ae_plain p
 
-val ae_message_unwrap: protected_ae_plain -> protected_hpke_plain
-let ae_message_unwrap p =
-  if honest p.i then
+val ae_message_unwrap: #i:id -> protected_ae_plain i -> Tot protected_hpke_plain
+let ae_message_unwrap #i p =
+  if honest i then
     p.p
   else 
     PlainHPKE.coerce p.p
-  
   
 (**
    We allow a transition from protected_ae_plain to ae_plain only if either there is no
    idealization or if if the message is not honest.
 *)
-val repr: p:protected_ae_plain{not ae_ind_cca || not (honest p.i)} -> Tot ae_plain
-let repr p = 
-  if honest p.i then
-    PlainHPKE.repr p.p
+val repr: #i:id -> p:protected_ae_plain i{not ae_ind_cca || not (honest i)} -> Tot ae_plain
+let repr #i p = 
+  if honest i then
+    PlainHPKE.repr p.p 
   else
     p.p
 
 (**
    Coerced messages can only be flagged as not honest.
 *)
-val coerce: #i:id{not ae_int_ctxt || not (honest i)} -> p:ae_plain -> Tot protected_ae_plain
+val coerce: #i:id -> p:ae_plain{not ae_int_ctxt || not (honest i)} -> Tot (protected_ae_plain i)
 let coerce #i p = 
   if honest i then
     let coerced_p = PlainHPKE.coerce p in
@@ -59,12 +59,9 @@ let coerce #i p =
   else
     Protected_ae_plain #i p
   
-val length: protected_ae_plain -> Tot nat
-let length p = 
-  if honest p.i then
+val length: #i:id -> (protected_ae_plain i) -> Tot nat
+let length #i p = 
+  if honest i then
     PlainHPKE.length p.p
   else
     length p.p
-
-val getIndex: protected_ae_plain -> Tot id
-let getIndex p = p.i
