examples/crypto/HyE.RSA.fst
@@ -20,8 +20,11 @@ open CoreCrypto
 
 module B = Platform.Bytes
 
-assume type pkey
-assume type skey
+assume val pk_size : nat
+assume val sk_size : nat
+
+type pkey = lbytes pk_size
+type skey = lbytes sk_size
 
 let plainsize  = aeadKeySize AES_128_GCM
 assume val ciphersize : nat
@@ -31,9 +34,16 @@ type cipher  = lbytes ciphersize
 type keypair = pkey * skey
 assume val generated : keypair -> Tot bool
 
-assume val gen: unit -> x:keypair{generated x}
+assume val gen: unit -> ST keypair
+  (requires (fun h0 -> True))
+  (ensures (fun h0 x h1 -> b2t (generated x)))
 assume val dec: skey -> cipher -> Tot (option plain)  (* this function is pure *)
-assume val enc: pk:pkey -> t:plain -> c:cipher { forall sk. generated (pk, sk) ==> dec sk c=Some t }  (* functional correctness *)
-assume val pkbytes: pkey -> bytes
+assume val enc: pk:pkey -> t:plain -> ST cipher 
+  (requires (fun h0 -> True))
+  (ensures (fun h0 c h1 -> 
+    (forall sk. generated (pk, sk) ==> dec sk c=Some t  (* functional correctness *))
+    /\ modifies_none h0 h1
+    ))
+assume val pkbytes: pkey -> Tot bytes
 assume val dummy: plain
 
